SP1Operations/AddOperation.lean
@@ -1,79 +1,98 @@
 import SP1Foundations
 
--- AddOperaton is not parameterized by a type `T` with `value` being `Word T`
--- because AddOperation is used only under the assumption that its input and
--- output limbs are all U16s.
--- @[aesop safe cases]
-structure AddOperation where
-  value : Word U16
-
 namespace AddOperation
 
-@[simp] lemma value_mk (value : Word U16) : (AddOperation.mk value).value = value := rfl
+/- @[simp] lemma value_mk (value : Word U16) : (AddOperation.mk value).value = value := rfl -/
 
 def spec
-  (cols : AddOperation)
-  (a : Word U16)
-  (b : Word U16)
+  (a0 a1 : U16)
+  (b0 b1 : U16)
+  (c0 c1 : U16)
   (is_real : U1) : Prop :=
-    is_real = 1 →
-    a.toBV32_U16 + b.toBV32_U16 = cols.value.toBV32_U16
+    is_real = 1 → BitVec.ofU16 a0 a1 = BitVec.ofU16 b0 b1 + BitVec.ofU16 c0 c1
 
-def constraints (cols : AddOperation)
-    (a b : Word U16) (is_real : U1) : Finset SP1Constraint :=
-  {
-     .assertZero (is_real * ((((a[0] + b[0]) - cols.value[0]) + (0 : BabyBear)) * (2013235201 : BabyBear)) * (((((a[0] + b[0]) - cols.value[0]) + 0) * 2013235201) - 1)),
-     .assertZero (is_real * ((((a[1] + b[1]) - cols.value[1]) + ((((a[0] + b[0]) - cols.value[0]) + (0 : BabyBear)) * (2013235201 : BabyBear))) * (2013235201 : BabyBear)) * (((((a[1] + b[1]) - cols.value[1]) + ((((a[0] + b[0]) - cols.value[0]) + 0) * 2013235201)) * 2013235201) - 1))
+def constraints
+  (I : Vector BabyBear 7)
+  : Finset SP1Constraint :=
+  let E0 := I[6] - 1
+  let E2 := I[6] * E0
+  let E4 := I[0] + I[2]
+  let E6 := E4 - I[4]
+  let E8 := E6 + 0
+  let E10 := E8 * 2013235201
+  let E12 := E10 - 1
+  let E14 := E10 * E12
+  let E16 := I[6] * E14
+  let E18 := I[1] + I[3]
+  let E20 := E18 - I[5]
+  let E22 := E20 + E10
+  let E24 := E22 * 2013235201
+  let E26 := E24 - 1
+  let E28 := E24 * E26
+  let E30 := I[6] * E28
+  { .assertZero E2
+  , .assertZero E16
+  , .assertZero E30
+  , .send (.byte (ByteOpcode.ofNat 6) I[4] 16 0) I[6]
+  , .send (.byte (ByteOpcode.ofNat 6) I[5] 16 0) I[6]
   }
 
 def constraints'
-    (cols : AddOperation)
-    (a : Word U16)
-    (b : Word U16)
-    (is_real : U1): Prop :=
-  let carry0 : BabyBear := 0
-  let carry1 : BabyBear := (a[0] + b[0] - cols.value[0] + carry0) * (baseInv : BabyBear)
-  let carry2 : BabyBear := (a[1] + b[1] - cols.value[1] + carry1) * (baseInv : BabyBear)
-  (is_real * carry1 * (carry1 - 1)) = 0 ∧
-  (is_real * carry2 * (carry2 - 1)) = 0
+  (I : Vector BabyBear 7)
+  : Prop :=
+  let carry0  : BabyBear := 0
+  let carry1  : BabyBear := (I[0] + I[2] - I[4] + carry0) * (baseInv : BabyBear)
+  let carry2  : BabyBear := (I[1] + I[3] - I[5] + carry1) * (baseInv : BabyBear)
+  I[6] = 0 ∨ (
+    I[6] = 1 ∧
+    (carry1 = 0 ∨ carry1 = 1) ∧
+    (carry2 = 0 ∨ carry2 = 1) ∧
+    (I[4] < 65536) ∧
+    (I[5] < 65536)
+  )
 
 def constraints_iff_constraints'
-    (cols : AddOperation)
-    (a : Word U16)
-    (b : Word U16)
-    (is_real : U1) :
-    constraintSet_toProp (cols.constraints a b is_real) ↔ cols.constraints' a b is_real:= by
+  (I : Vector BabyBear 7)
+  : constraintSet_toProp (constraints I) ↔ constraints' I := by
   simp [constraints, constraints']
+  simp [ByteOpcode.ofNat, Nat.ble, Nat.beq, ByteOpcode.constrain]
+  simp [sub_eq_zero]
+  sorry
 
 theorem correct
-    (cols : AddOperation)
-    (a : Word U16) (b : Word U16)
-    (is_real : U1) :
-    constraintSet_toProp (cols.constraints a b is_real) → cols.spec a b is_real := by
-  rw [constraints_iff_constraints']
-  intro ⟨q1, q2⟩
+  (a0 a1 : U16)
+  (b0 b1 : U16)
+  (c0 c1 : U16)
+  (is_real : U1) :
+    constraintSet_toProp (constraints #v[b0, b1, c0, c1, a0, a1, is_real]) →
+    spec a0 a1 b0 b1 c0 c1 is_real := by
+  rw [constraints_iff_constraints' (#v[b0, b1, c0, c1, a0, a1, is_real])]
+  simp [constraints', spec]
+  intro q1
 
-  -- Since is_real = 1, substitute and apply 1 * x = x to get original constraints
   intro h_is_real
-  simp [h_is_real, sub_eq_zero, mul_eq_zero] at q1 q2
-  simp [Word.toBV32_U16, BitVec.ofNatLT, Fin.add_def]
+  simp [h_is_real] at q1
 
-  let i1 := a[0].in_range
-  let i2 := a[1].in_range
-  let i3 := b[0].in_range
-  let i4 := b[1].in_range
-  let i5 := cols.value[0].in_range
-  let i6 := cols.value[1].in_range
+  let ⟨qq1, ⟨qq2, ⟨qq3, aa4⟩⟩⟩ := q1
+  clear q1
+  simp [sub_eq_zero, mul_eq_zero] at qq1 qq2
+  simp [BitVec.ofU16, BitVec.ofNatLT]
 
-  -- Cases on whether the lower limb led to a carry or not
-  cases q1 with
-  | inl qq1 =>
-      rw [qq1] at q2
+  let i0 := c0.in_range
+  let i1 := c1.in_range
+  let i2 := b0.in_range
+  let i3 := b1.in_range
+
+  cases qq1 with
+  | inl qqq1 =>
+      rw [qqq1] at qq2
       simp [Fin.mul_def, Fin.sub_def, Fin.add_def, Fin.ext_iff, BabyBearPrime] at *
-      omega
-  | inr qq1 =>
-      rw [qq1] at q2
+      rw [Fin.lt_def] at qq3 aa4
+      aesop (add 50% tactic (by omega))
+  | inr qqq1 =>
+      rw [qqq1] at qq2
       simp [Fin.mul_def, Fin.sub_def, Fin.add_def, Fin.ext_iff, BabyBearPrime] at *
-      omega
+      rw [Fin.lt_def] at qq3 aa4
+      aesop (add 50% tactic (by omega))
 
 end AddOperation
